Weidenbach_Book/CDCL_Two_Watched_Literals_Invariant.thy
@@ -1,0 +1,463 @@
+(*  Title: Implementation of CDCL with Two Watched Literals
+    Author: Mathias Fleury <mathias.fleury@mpi-inf.mpg.de>
+*)
+
+section \<open>Implementation for 2 Watched-Literals\<close>
+
+theory CDCL_Two_Watched_Literals_Invariant
+imports CDCL_Two_Watched_Literals DPLL_CDCL_W_Implementation
+begin
+
+subsection \<open>Interpretation for @{term conflict_driven_clause_learning\<^sub>W.cdcl\<^sub>W}\<close>
+
+text \<open>We define here the 2-WL with the invariant and show the role of the candidates.\<close>
+context abstract_twl
+begin
+
+subsubsection \<open>Direct Interpretation\<close>
+lemma mset_map_removeAll_cond:
+  "mset (map (\<lambda>x. mset (raw_clause x))
+    (removeAll_cond (\<lambda>D. mset (raw_clause D) = mset (raw_clause C)) N))
+  = mset (removeAll (mset (raw_clause C)) (map (\<lambda>x. mset (raw_clause x)) N))"
+  by (induction N) auto
+
+lemma mset_raw_init_clss_init_state:
+  "mset (map (\<lambda>x. mset (raw_clause x)) (raw_init_clss (init_state (map raw_clause N))))
+  = mset (map (\<lambda>x. mset (raw_clause x)) N)"
+  by (metis (no_types, lifting) init_clss_init_state map_eq_conv map_map o_def)
+
+interpretation rough_cdcl: state\<^sub>W
+  "\<lambda>C. mset (raw_clause C)"
+    (* does not matter if the invariants do not hold *)
+  "\<lambda>L C. TWL_Clause (watched C) (L # unwatched C)"
+  "\<lambda>L C. TWL_Clause [] (remove1 L (raw_clause C))"
+  "\<lambda>C. clauses_of_l (map raw_clause C)" "op @"
+  "\<lambda>L C. L \<in> set C" "op #" "\<lambda>C. remove1_cond (\<lambda>D. mset (raw_clause D) = mset (raw_clause C))"
+
+  mset "\<lambda>xs ys. case_prod append (fold (\<lambda>x (ys, zs). (remove1 x ys, x # zs)) xs (ys, []))"
+  "op #" remove1
+
+  raw_clause "\<lambda>C. TWL_Clause [] C"
+  trail "\<lambda>S. hd (raw_trail S)"
+  raw_init_clss raw_learned_clss backtrack_lvl raw_conflicting
+  cons_trail tl_trail "\<lambda>C. add_init_cls (raw_clause C)" "\<lambda>C. add_learned_cls (raw_clause C)"
+  "\<lambda>C. remove_cls (raw_clause C)"
+  update_backtrack_lvl
+  update_conflicting "\<lambda>N. init_state (map raw_clause N)" restart'
+  apply unfold_locales
+  apply (case_tac "raw_trail S")
+  apply (simp_all add: add_init_cls_def add_learned_cls_def clause_rewatch clause_watch
+    cons_trail_def remove_cls_def restart'_def tl_trail_def map_tl comp_def
+    ac_simps mset_map_removeAll_cond mset_raw_init_clss_init_state)
+
+  apply (auto simp: mset_map image_mset_subseteq_mono[OF restart_learned] )
+  done
+
+interpretation rough_cdcl: conflict_driven_clause_learning\<^sub>W
+  "\<lambda>C. mset (raw_clause C)"
+    (* does not matter if the invariants do not hold *)
+  "\<lambda>L C. TWL_Clause (watched C) (L # unwatched C)"
+  "\<lambda>L C. TWL_Clause [] (remove1 L (raw_clause C))"
+  "\<lambda>C. clauses_of_l (map raw_clause C)" "op @"
+  "\<lambda>L C. L \<in> set C" "op #" "\<lambda>C. remove1_cond (\<lambda>D. mset (raw_clause D) = mset (raw_clause C))"
+
+  mset "\<lambda>xs ys. case_prod append (fold (\<lambda>x (ys, zs). (remove1 x ys, x # zs)) xs (ys, []))"
+  "op #" remove1
+
+  "\<lambda>C. raw_clause C" "\<lambda>C. TWL_Clause [] C"
+  trail "\<lambda>S. hd (raw_trail S)"
+  raw_init_clss raw_learned_clss backtrack_lvl raw_conflicting
+  cons_trail tl_trail "\<lambda>C. add_init_cls (raw_clause C)" "\<lambda>C. add_learned_cls (raw_clause C)"
+  "\<lambda>C. remove_cls (raw_clause C)"
+  update_backtrack_lvl
+  update_conflicting "\<lambda>N. init_state (map raw_clause N)" restart'
+  by unfold_locales
+ 
+declare local.rough_cdcl.mset_ccls_ccls_of_cls[simp del]
+
+subsubsection \<open>Opaque Type with Invariant\<close>
+
+declare rough_cdcl.state_simp[simp del]
+
+definition cons_trail_twl :: "('v, nat, 'v twl_clause) marked_lit \<Rightarrow> 'v wf_twl \<Rightarrow> 'v wf_twl"
+  where
+"cons_trail_twl L S \<equiv> twl_of_rough_state (cons_trail L (rough_state_of_twl S))"
+
+lemma wf_twl_state_cons_trail:
+  assumes
+    undef: "undefined_lit (trail S) (lit_of L)" and
+    wf: "wf_twl_state S"
+  shows "wf_twl_state (cons_trail L S)"
+  using undef wf wf_rewatch[of S "mmset_of_mlit' L"] unfolding wf_twl_state_def Ball_def
+  by (auto simp: cons_trail_def defined_lit_map comp_def image_def twl.raw_clauses_def)
+
+lemma rough_state_of_twl_cons_trail:
+  "undefined_lit (trail_twl S) (lit_of L) \<Longrightarrow>
+    rough_state_of_twl (cons_trail_twl L S) = cons_trail L (rough_state_of_twl S)"
+  using rough_state_of_twl twl_of_rough_state_inverse wf_twl_state_cons_trail
+  unfolding cons_trail_twl_def by blast
+
+abbreviation add_init_cls_twl where
+"add_init_cls_twl C S \<equiv> twl_of_rough_state (add_init_cls C (rough_state_of_twl S))"
+
+lemma wf_twl_add_init_cls: "wf_twl_state S \<Longrightarrow> wf_twl_state (add_init_cls L S)"
+  unfolding wf_twl_state_def by (auto simp: wf_watch add_init_cls_def comp_def twl.raw_clauses_def
+    split: if_split_asm)
+
+lemma rough_state_of_twl_add_init_cls:
+  "rough_state_of_twl (add_init_cls_twl L S) = add_init_cls L (rough_state_of_twl S)"
+  using rough_state_of_twl twl_of_rough_state_inverse wf_twl_add_init_cls by blast
+
+abbreviation add_learned_cls_twl where
+"add_learned_cls_twl C S \<equiv> twl_of_rough_state (add_learned_cls C (rough_state_of_twl S))"
+
+lemma wf_twl_add_learned_cls: "wf_twl_state S \<Longrightarrow> wf_twl_state (add_learned_cls L S)"
+  unfolding wf_twl_state_def by (auto simp: wf_watch add_learned_cls_def twl.raw_clauses_def
+    split: if_split_asm)
+
+lemma rough_state_of_twl_add_learned_cls:
+  "rough_state_of_twl (add_learned_cls_twl L S) = add_learned_cls L (rough_state_of_twl S)"
+  using rough_state_of_twl twl_of_rough_state_inverse wf_twl_add_learned_cls by blast
+
+abbreviation remove_cls_twl where
+"remove_cls_twl C S \<equiv> twl_of_rough_state (remove_cls C (rough_state_of_twl S))"
+
+lemma set_removeAll_condD: "x \<in> set (removeAll_cond f xs) \<Longrightarrow> x \<in> set xs"
+  by (induction xs) (auto split: if_split_asm)
+
+lemma wf_twl_remove_cls: "wf_twl_state S \<Longrightarrow> wf_twl_state (remove_cls L S)"
+  unfolding wf_twl_state_def by (auto simp: wf_watch remove_cls_def twl.raw_clauses_def comp_def
+    split: if_split_asm dest: set_removeAll_condD)  
+
+lemma rough_state_of_twl_remove_cls:
+  "rough_state_of_twl (remove_cls_twl L S) = remove_cls L (rough_state_of_twl S)"
+  using rough_state_of_twl twl_of_rough_state_inverse wf_twl_remove_cls by blast
+
+abbreviation init_state_twl where
+"init_state_twl N \<equiv> twl_of_rough_state (init_state N)"
+
+lemma wf_twl_state_wf_twl_state_fold_add_init_cls:
+  assumes "wf_twl_state S"
+  shows "wf_twl_state (fold add_init_cls N S)"
+  using assms apply (induction N arbitrary: S)
+   apply (auto simp: wf_twl_state_def)[]
+  by (simp add: wf_twl_add_init_cls)
+
+lemma wf_twl_state_epsilon_state[simp]:
+  "wf_twl_state (TWL_State [] [] [] 0 None)"
+  by (auto simp: wf_twl_state_def twl.raw_clauses_def)
+
+lemma wf_twl_init_state: "wf_twl_state (init_state N)"
+  unfolding init_state_def by (auto intro!: wf_twl_state_wf_twl_state_fold_add_init_cls)
+
+lemma rough_state_of_twl_init_state:
+  "rough_state_of_twl (init_state_twl N) = init_state N"
+  by (simp add: twl_of_rough_state_inverse wf_twl_init_state)
+
+abbreviation tl_trail_twl where
+"tl_trail_twl S \<equiv> twl_of_rough_state (tl_trail (rough_state_of_twl S))"
+
+lemma wf_twl_state_tl_trail: "wf_twl_state S \<Longrightarrow> wf_twl_state (tl_trail S)"
+  by (auto simp add: twl_of_rough_state_inverse wf_twl_init_state wf_twl_cls_wf_twl_cls_tl
+    tl_trail_def wf_twl_state_def distinct_tl map_tl comp_def twl.raw_clauses_def)
+
+lemma rough_state_of_twl_tl_trail:
+  "rough_state_of_twl (tl_trail_twl S) = tl_trail (rough_state_of_twl S)"
+  using rough_state_of_twl twl_of_rough_state_inverse wf_twl_state_tl_trail by blast
+
+abbreviation update_backtrack_lvl_twl where
+"update_backtrack_lvl_twl k S \<equiv> twl_of_rough_state (update_backtrack_lvl k (rough_state_of_twl S))"
+
+lemma wf_twl_state_update_backtrack_lvl:
+  "wf_twl_state S \<Longrightarrow> wf_twl_state (update_backtrack_lvl k S)"
+  unfolding wf_twl_state_def by (auto simp: comp_def twl.raw_clauses_def)
+
+lemma rough_state_of_twl_update_backtrack_lvl:
+  "rough_state_of_twl (update_backtrack_lvl_twl k S) = update_backtrack_lvl k
+    (rough_state_of_twl S)"
+  using rough_state_of_twl twl_of_rough_state_inverse wf_twl_state_update_backtrack_lvl by fast
+
+abbreviation update_conflicting_twl where
+"update_conflicting_twl k S \<equiv> twl_of_rough_state (update_conflicting k (rough_state_of_twl S))"
+
+lemma wf_twl_state_update_conflicting:
+  "wf_twl_state S \<Longrightarrow> wf_twl_state (update_conflicting k S)"
+  unfolding wf_twl_state_def by (auto simp: twl.raw_clauses_def comp_def)
+
+lemma rough_state_of_twl_update_conflicting:
+  "rough_state_of_twl (update_conflicting_twl k S) = update_conflicting k
+    (rough_state_of_twl S)"
+  using rough_state_of_twl twl_of_rough_state_inverse wf_twl_state_update_conflicting by fast
+
+abbreviation raw_clauses_twl where
+"raw_clauses_twl S \<equiv> twl.raw_clauses (rough_state_of_twl S)"
+
+abbreviation restart_twl where
+"restart_twl S \<equiv> twl_of_rough_state (restart' (rough_state_of_twl S))"
+lemma mset_union_mset_setD:
+  "mset A \<subseteq># mset B \<Longrightarrow> set A \<subseteq> set B"
+  by auto
+
+lemma wf_wf_restart': "wf_twl_state S \<Longrightarrow> wf_twl_state (restart' S)"
+  unfolding restart'_def wf_twl_state_def apply standard
+   apply clarify
+   apply (rename_tac x)
+   apply (subgoal_tac "wf_twl_cls (trail S) x")
+    apply (case_tac x)
+  using restart_learned by (auto simp: twl.raw_clauses_def comp_def dest: mset_union_mset_setD)
+
+lemma rough_state_of_twl_restart_twl:
+  "rough_state_of_twl (restart_twl S) = restart' (rough_state_of_twl S)"
+  by (simp add: twl_of_rough_state_inverse wf_wf_restart')
+ 
+sublocale conflict_driven_clause_learning\<^sub>W
+  "\<lambda>C. mset (raw_clause C)"
+    (* does not matter if the invariants do not hold *)
+  "\<lambda>L C. TWL_Clause (watched C) (L # unwatched C)"
+  "\<lambda>L C. TWL_Clause [] (remove1 L (raw_clause C))"
+  "\<lambda>C. clauses_of_l (map raw_clause C)" "op @"
+  "\<lambda>L C. L \<in> set C" "op #" "\<lambda>C. remove1_cond (\<lambda>D. mset (raw_clause D) = mset (raw_clause C))"
+
+  mset "\<lambda>xs ys. case_prod append (fold (\<lambda>x (ys, zs). (remove1 x ys, x # zs)) xs (ys, []))"
+  "op #" remove1
+
+  "\<lambda>C. raw_clause C" "\<lambda>C. TWL_Clause [] C"
+  trail_twl "\<lambda>S. hd (raw_trail_twl S)"
+  raw_init_clss_twl
+  raw_learned_clss_twl
+  backtrack_lvl_twl
+  raw_conflicting_twl
+  cons_trail_twl
+  tl_trail_twl
+  "\<lambda>C. add_init_cls_twl (raw_clause C)"
+  "\<lambda>C. add_learned_cls_twl (raw_clause C)"
+  "\<lambda>C. remove_cls_twl (raw_clause C)"
+  update_backtrack_lvl_twl
+  update_conflicting_twl
+  "\<lambda>N. init_state_twl (map raw_clause N)"
+  restart_twl
+  apply unfold_locales
+           using rough_cdcl.hd_raw_trail apply blast
+         apply (simp_all add: rough_state_of_twl_cons_trail rough_state_of_twl_tl_trail
+           rough_state_of_twl_add_init_cls rough_state_of_twl_add_learned_cls
+           rough_state_of_twl_remove_cls rough_state_of_twl_update_backtrack_lvl
+           rough_state_of_twl_update_conflicting)[7]
+       using rough_cdcl.init_clss_cons_trail rough_cdcl.init_clss_tl_trail 
+       rough_cdcl.init_clss_add_init_cls rough_cdcl.init_clss_remove_cls
+       rough_cdcl.init_clss_add_learned_cls
+       rough_cdcl.init_clss_update_backtrack_lvl
+       rough_cdcl.init_clss_update_conflicting
+       apply (auto simp add: rough_state_of_twl_cons_trail rough_state_of_twl_tl_trail
+         rough_state_of_twl_add_init_cls rough_state_of_twl_add_learned_cls
+         rough_state_of_twl_remove_cls rough_state_of_twl_update_backtrack_lvl
+         rough_state_of_twl_update_conflicting comp_def)[7]
+       using rough_cdcl.learned_clss_cons_trail rough_cdcl.learned_clss_tl_trail 
+       rough_cdcl.learned_clss_add_init_cls rough_cdcl.learned_clss_remove_cls
+       rough_cdcl.learned_clss_add_learned_cls
+       rough_cdcl.learned_clss_update_backtrack_lvl
+       rough_cdcl.learned_clss_update_conflicting
+       apply (auto simp add: rough_state_of_twl_cons_trail rough_state_of_twl_tl_trail
+         rough_state_of_twl_add_init_cls rough_state_of_twl_add_learned_cls
+         rough_state_of_twl_remove_cls rough_state_of_twl_update_backtrack_lvl
+         rough_state_of_twl_update_conflicting comp_def)[7]
+      apply (auto simp add: rough_state_of_twl_cons_trail rough_state_of_twl_tl_trail
+        rough_state_of_twl_add_init_cls rough_state_of_twl_add_learned_cls
+        rough_state_of_twl_remove_cls rough_state_of_twl_update_backtrack_lvl
+        rough_state_of_twl_update_conflicting comp_def)[14]  
+    using init_clss_init_state apply (auto simp: rough_state_of_twl_init_state)[5]
+  using rough_cdcl.init_clss_restart_state rough_cdcl.learned_clss_restart_state 
+  apply (auto simp: rough_state_of_twl_restart_twl)[5]
+  done
+ 
+declare local.rough_cdcl.mset_ccls_ccls_of_cls[simp del]
+abbreviation state_eq_twl (infix "\<sim>TWL" 51) where
+"state_eq_twl S S' \<equiv> rough_cdcl.state_eq (rough_state_of_twl S) (rough_state_of_twl S')"
+notation state_eq (infix "\<sim>" 51)
+declare state_simp[simp del]
+
+text \<open>To avoid ambiguities:\<close>
+no_notation state_eq_twl (infix "\<sim>" 51)
+
+inductive propagate_twl :: "'v wf_twl \<Rightarrow> 'v wf_twl \<Rightarrow> bool" where
+propagate_twl_rule: "(L, C) \<in> candidates_propagate_twl S \<Longrightarrow>
+  S' \<sim> cons_trail_twl (Propagated L C) S \<Longrightarrow>
+  raw_conflicting_twl S = None \<Longrightarrow>
+  propagate_twl S S'"
+  
+inductive_cases propagate_twlE: "propagate_twl S T"  
+thm propagateE
+
+lemma distinct_filter_eq_if:
+  "distinct C \<Longrightarrow> length (filter (op = L) C) = (if L \<in> set C then 1 else 0)"
+  by (induction C) auto
+
+lemma distinct_mset_remove1_All:
+  "distinct_mset C \<Longrightarrow> remove1_mset L C = removeAll_mset L C"
+  by (auto simp: multiset_eq_iff distinct_mset_count_less_1)
+
+lemma propagate_twl_iff_propagate:                    
+  assumes inv: "cdcl\<^sub>W_all_struct_inv S"
+  shows "propagate S T \<longleftrightarrow> propagate_twl S T" (is "?P \<longleftrightarrow> ?T")
+proof
+  assume ?P
+  then obtain L E where
+    "raw_conflicting_twl S = None" and
+    CL_Clauses: "E \<in> set (twl.raw_clauses S)" and
+    LE: "L \<in># mset (raw_clause E)" and
+    tr_CNot: "trail_twl S \<Turnstile>as CNot (remove1_mset L (mset (raw_clause E)))" and
+    undef_lot[simp]: "undefined_lit (trail_twl S) L" and
+    "T \<sim> cons_trail_twl (Propagated L E) S"
+     by (blast elim: propagateE)
+  have "distinct (raw_clause E)"
+    using inv CL_Clauses unfolding cdcl\<^sub>W_all_struct_inv_def distinct_mset_set_def
+    distinct_cdcl\<^sub>W_state_def raw_clauses_def by auto
+  then have X: "remove1_mset L (mset (raw_clause E)) = mset_set (set (raw_clause E) - {L})"
+    by (auto simp: multiset_eq_iff raw_clause_def count_mset distinct_filter_eq_if)
+  have "(L, E) \<in> candidates_propagate_twl S"
+    apply (rule wf_candidates_propagate_complete)
+         using rough_state_of_twl apply auto[]
+        using CL_Clauses unfolding raw_clauses_def twl.raw_clauses_def
+        apply auto[]
+       using LE apply simp
+      using tr_CNot X apply simp
+     using undef_lot apply blast
+     done
+  show ?T 
+    apply (rule propagate_twl_rule)
+       apply (rule \<open>(L, E) \<in> candidates_propagate_twl S\<close>)
+      using \<open>T \<sim> cons_trail_twl (Propagated L E) S\<close>
+      apply (auto simp: \<open>raw_conflicting_twl S = None\<close> twl.state_eq_def)
+    done
+next
+  assume ?T
+  then obtain L C where
+    LC: "(L, C) \<in> candidates_propagate_twl S" and
+    T: "T \<sim> cons_trail_twl (Propagated L C) S" and
+    confl: "raw_conflicting_twl S = None"
+    by (auto elim: propagate_twlE)
+  have
+    C'S: "C \<in> set (raw_clauses_twl S)" and
+    L: "set (watched C) - uminus ` lits_of_l (trail_twl S) = {L}" and
+    undef: "undefined_lit (trail_twl S) L"
+    using LC unfolding candidates_propagate_def raw_clauses_def by auto
+  have dist: "distinct (raw_clause C)"
+    using inv C'S unfolding cdcl\<^sub>W_all_struct_inv_def distinct_cdcl\<^sub>W_state_def
+     distinct_mset_set_def twl.raw_clauses_def by fastforce
+  then have C_L_L: "mset_set (set (raw_clause C) - {L}) = mset (raw_clause C) - {#L#}"
+    by (metis distinct_mset_distinct distinct_mset_minus distinct_mset_set_mset_ident mset_remove1
+      set_mset_mset set_remove1_eq)
+    
+  show ?P
+    apply (rule propagate_rule[of S C L])
+        using confl apply auto[]
+       using C'S unfolding twl.raw_clauses_def apply (simp add: raw_clauses_def)
+       using L unfolding candidates_propagate_def apply (auto simp: raw_clause_def)[]
+      using wf_candidates_propagate_sound[OF _ LC] rough_state_of_twl dist
+      apply (simp add: distinct_mset_remove1_All)
+     using undef apply simp
+    using T undef by (smt backtrack_lvl_cons_trail confl init_clss_cons_trail 
+      learned_clss_cons_trail marked_lit.sel(2) raw_conflicting_cons_trail state_eq_def 
+      trail_cons_trail twl2.mmset_of_mlit.simps(1) twl2.mset_cls_cls_of_ccls)
+qed
+
+no_notation twl.state_eq_twl (infix "\<sim>TWL" 51)
+
+inductive conflict_twl where
+conflict_twl_rule:
+"C \<in> candidates_conflict_twl S \<Longrightarrow>
+  S' \<sim> update_conflicting_twl (Some (raw_clause C)) S \<Longrightarrow>
+  raw_conflicting_twl S = None \<Longrightarrow>
+  conflict_twl S S'"
+
+inductive_cases conflict_twlE: "conflict_twl S T"
+
+lemma conflict_twl_iff_conflict:
+  shows "conflict S T \<longleftrightarrow> conflict_twl S T" (is "?C \<longleftrightarrow> ?T")
+proof
+  assume ?C
+  then obtain D where
+    S: "raw_conflicting_twl S = None" and
+    D: "D \<in> set (raw_clauses S)" and
+    MD: "trail_twl S \<Turnstile>as CNot (mset (raw_clause D))" and
+    T: "T \<sim> update_conflicting_twl (Some (raw_clause D)) S"
+    by (elim conflictE)
+    
+  have "D \<in> candidates_conflict_twl S"
+    apply (rule wf_candidates_conflict_complete)
+       apply simp
+      using D apply (auto simp: raw_clauses_def twl.raw_clauses_def)[]
+    using MD S by auto
+  moreover have "T \<sim> twl_of_rough_state (update_conflicting (Some (raw_clause D)) 
+  (rough_state_of_twl S))"
+    using T unfolding rough_cdcl.state_eq_def state_eq_def by auto
+  ultimately show ?T
+    using S by (auto intro: conflict_twl_rule)
+next
+  assume ?T
+  then obtain C where
+    C: "C \<in> candidates_conflict_twl S" and
+    T: "T \<sim> update_conflicting_twl (Some (raw_clause C)) S" and
+    confl: "raw_conflicting_twl S = None"
+    by (auto elim: conflict_twlE)
+  have
+    "C \<in> set (raw_clauses S)"
+    using C unfolding candidates_conflict_def raw_clauses_def twl.raw_clauses_def by auto
+ moreover have "trail_twl S \<Turnstile>as CNot (mset (raw_clause C))"
+    using wf_candidates_conflict_sound[OF _ C] by auto
+ ultimately show ?C apply -
+   apply (rule conflict.conflict_rule[of _ C])
+   using confl T unfolding rough_cdcl.state_eq_def by (auto simp del: map_map)
+qed
+
+inductive cdcl\<^sub>W_twl :: "'v wf_twl \<Rightarrow> 'v wf_twl \<Rightarrow> bool" for S :: "'v wf_twl" where
+propagate: "propagate_twl S S' \<Longrightarrow> cdcl\<^sub>W_twl S S'" |
+conflict: "conflict_twl S S' \<Longrightarrow> cdcl\<^sub>W_twl S S'" |
+other: "cdcl\<^sub>W_o S S' \<Longrightarrow> cdcl\<^sub>W_twl S S'"|
+rf: "cdcl\<^sub>W_rf S S' \<Longrightarrow> cdcl\<^sub>W_twl S S'"
+
+lemma cdcl\<^sub>W_twl_iff_cdcl\<^sub>W:
+  assumes "cdcl\<^sub>W_all_struct_inv S"
+  shows "cdcl\<^sub>W_twl S T \<longleftrightarrow> cdcl\<^sub>W S T"
+  by (simp add: assms cdcl\<^sub>W.simps cdcl\<^sub>W_twl.simps conflict_twl_iff_conflict
+    propagate_twl_iff_propagate del: map_map)
+
+lemma rtranclp_cdcl\<^sub>W_twl_all_struct_inv_inv:
+  assumes "cdcl\<^sub>W_twl\<^sup>*\<^sup>* S T" and "cdcl\<^sub>W_all_struct_inv S"
+  shows "cdcl\<^sub>W_all_struct_inv T"
+  using assms by (induction rule: rtranclp_induct)
+  (simp_all add: cdcl\<^sub>W_twl_iff_cdcl\<^sub>W cdcl\<^sub>W_all_struct_inv_inv del: map_map)
+
+lemma rtranclp_cdcl\<^sub>W_twl_iff_rtranclp_cdcl\<^sub>W:
+  assumes "cdcl\<^sub>W_all_struct_inv S"
+  shows "cdcl\<^sub>W_twl\<^sup>*\<^sup>* S T \<longleftrightarrow> cdcl\<^sub>W\<^sup>*\<^sup>* S T" (is "?T \<longleftrightarrow> ?W")
+proof
+  assume ?W
+  then show ?T
+    proof (induction rule: rtranclp_induct)
+      case base
+      then show ?case by simp
+    next
+      case (step T U) note st = this(1) and cdcl = this(2) and IH = this(3)
+      have "cdcl\<^sub>W_twl T U"
+        using assms st cdcl rtranclp_cdcl\<^sub>W_all_struct_inv_inv cdcl\<^sub>W_twl_iff_cdcl\<^sub>W
+        by blast
+      then show ?case using IH by auto
+    qed
+next
+  assume ?T
+  then show ?W
+    proof (induction rule: rtranclp_induct)
+      case base
+      then show ?case by simp
+    next
+      case (step T U) note st = this(1) and cdcl = this(2) and IH = this(3)
+      have "cdcl\<^sub>W T U"
+        using assms st cdcl rtranclp_cdcl\<^sub>W_twl_all_struct_inv_inv cdcl\<^sub>W_twl_iff_cdcl\<^sub>W
+        by blast
+      then show ?case using IH by auto
+    qed
+qed
+
+end
+
+end
